\section{Diskretisierung Regler}
Der Ausgang setzt sich aus den Anteilen $U_p$, $U_i$ und $U_d$ zusammen. 
\[ U[k] = U_p[k] + U_i[k] + U_d[k] \]

\subsection{P Anteil}
\[ H_p(s) = K_p \]
\[ H_p(z) = K_p \]
\[ U_p[k] = E_p[k] \cdot K_p \]

\subsection{I Anteil}
\[ H_i(s) = \frac{K_p}{T_i \cdot s} \]
Trapezregel
\[ s = \frac{2}{T} \cdot \frac{z - 1}{z + 1} \]
\[ H_i(z) = \frac{K_p}{T_i \cdot \dfrac{2}{T} \cdot \dfrac{z - 1}{z + 1}}
 = \frac{K_p \cdot T \cdot (z + 1)}{T_i \cdot 2 \cdot (z - 1)}
 = \frac{K_p \cdot T \cdot z + K_p \cdot T}{T_i \cdot 2 \cdot z - T_i \cdot 2}
 = \frac{K_p \cdot T + K_p \cdot T \cdot z^{-1}}{T_i \cdot 2 - T_i \cdot 2 \cdot z^{-1}}
 = \frac{U_i(z)}{E(z)} \]
\[ U_i(z) \cdot (T_i \cdot 2 - T_i \cdot 2 \cdot z^{-1})
 = E(z) \cdot (K_p \cdot T + K_p \cdot T \cdot z^{-1}) \]
\[ U_i[k] =  U_i[k-1] + \left(E[k] + E[k-1]\right) \cdot
 \underbrace{\frac{K_p \cdot T}{2 \cdot T_i}}_{K_i} \]

\subsection{I Anteil mit Anti-Reset Windup}
Rechnung gleich wie ohne ARW
\[ U_i[k] =  U_i[k-1] + \left(E[k] + E[k-1]\right) \cdot
 \underbrace{\frac{K_p \cdot T}{2 \cdot T_i}}_{K_i}
 + \left(U_{Sat}[k] - U[k] + U_{Sat}[k-1] - U[k-1]\right) \cdot
 \underbrace{\frac{T}{2 \cdot T_r}}_{K_r} \]

\subsection{D Anteil}
\[ H_d(s) = - \frac{T_d \cdot s}{\dfrac{T_d}{N} \cdot s + 1} \]
Rückwärtsrechteckregel
\[ s = \frac{z - 1}{t \cdot z} \]
\[ H_d(z) = -\frac{T_d \cdot \dfrac{z - 1}{t \cdot z}}{\dfrac{T_d}{N} \cdot \dfrac{z - 1}{t \cdot z} + 1}
 = -\frac{T_d \cdot N \cdot (z - 1)}{T_d \cdot (z - 1) + N \cdot t \cdot z}
 = -\frac{T_d \cdot N \cdot z - T_d \cdot N}{T_d \cdot z + N \cdot t \cdot z - T_d} \]
\[ H_d(z) = -\frac{T_d \cdot N - T_d \cdot N \cdot z^{-1}}{T_d + N \cdot t - T_d \cdot z^{-1}}
 = \frac{U_d(z)}{E(z)} \]
\[ U_d(z) \cdot (T_d + N \cdot t - T_d \cdot z^{-1})
 = - E(z) \cdot (T_d \cdot N - T_d \cdot N \cdot z^{-1}) \]
\[ U_d[k] = U_d[k-1] \cdot \frac{T_d}{T_d + N \cdot t}
 - \left(E[k] - E[k-1]\right) \cdot \frac{T_d}{T_d + N \cdot t} \cdot N \]
\[ U_d[k] = \underbrace{\frac{1}{1 + \dfrac{N \cdot t}{T_d}}}_{K_d} \cdot \left(U_d[k-1]
 - \left(E[k] - E[k-1]\right) \cdot N\right) \]
